add eorubfx hash and performance fix

src/main.ml
@@ -24,7 +24,7 @@ let serialize_dat (d:CFI.Rewriter.data) : Yojson.Basic.t =
     ("devs", `List (List.map ji d.devs));
     ("dsets", `List (List.map (fun d -> `List (List.map ji d)) d.dsets));
     ("tc", `List (List.map (fun ((h, tbl), ti) -> `Assoc [
-      ("hash", match h with H_UBFX (a, b) -> `List [ji a; ji b]);
+      ("hash", match h with H_UBFX (a, b) -> `List [ji a; ji b] | H_EOR_UBFX (a, b, c) -> `List [ji a; ji b; ji c]);
       ("tbl", `List (List.map ji tbl));
       ("ti", ji ti);
     ]) d.tc));
