theories/Hash.v
@@ -5,18 +5,23 @@ Import ListNotations.
 
 Section Hashing.
   Variant hash :=
-    | H_UBFX (lsb width: int).
+    | H_UBFX (lsb width: int)
+    | H_EOR_UBFX (shift lsb width: int).
   Definition hash_size h :=
     match h with
-    | H_UBFX lsb width => 1 << width
+    | H_UBFX _ width
+    | H_EOR_UBFX _ _ width =>
+        1 << width
     end.
   Definition hash_func h :=
     match h with
     | H_UBFX lsb width => λ v, (v >> lsb) mod (1 << width)
+    | H_EOR_UBFX shift lsb width => λ v, ((v lxor (v >> shift)) >> lsb) mod (1 << width)
     end.
   Definition hash_code h r :=
     match h with
     | H_UBFX lsb width => [Asm.UBFX true r r lsb width]
+    | H_EOR_UBFX shift lsb width => [Asm.EOR_lsr r r r shift; Asm.UBFX true r r lsb width]
     end.
   Fixpoint valid_hash h D D' s :=
     match D, D' with
@@ -29,34 +34,36 @@ Section Hashing.
              valid_hash h t t' s'
     | _, _ => true
     end.
-  Function find_ubfx_hash' width lsb D D' {measure to_nat lsb} :=
-    if (lsb <=? 0) then None
-    else if valid_hash (H_UBFX lsb width) D D' MSet.empty
-         then Some (H_UBFX lsb width)
-         else find_ubfx_hash' width (lsb-1) D D'.
-  Proof. lia. Defined.
-  Function find_ubfx_hash width D D' {measure (λ width, to_nat (33 - width)) width} :=
-    if (32 <=? width) || (width <? 0) then None
-    else match find_ubfx_hash' width 32 D D' with
-         | Some h => Some h
-         | None => find_ubfx_hash (width+1) D D'
-         end.
-  Proof. lia. Defined.
+  Section find_valid.
+    Variable max : int.
+    Function find_valid (f: int -> bool) x {measure (λ x, to_nat (max - x)) x} :=
+      if (x <? max) then
+        if (f x) then Some x else find_valid f (x+1)
+      else None.
+    Proof. lia. Defined.
+  End find_valid.
+  Definition issome {A} (x: option A) := if x then true else false.
+  Definition find_ubfx_lsb width D D' := find_valid 32 (λ lsb, valid_hash (H_UBFX lsb width) D D' MSet.empty) 0.
+  Definition find_ubfx_width D D' := find_valid 12 (λ width, issome (find_ubfx_lsb width D D')) 3.
+  Definition find_eorubfx_lsb shift width D D' := find_valid 32 (λ lsb, valid_hash (H_EOR_UBFX shift lsb width) D D' MSet.empty) 0.
+  Definition find_eorubfx_shift width D D' := find_valid 32 (λ shift, issome (find_eorubfx_lsb shift width D D')) 1.
+  Definition find_eorubfx_width D D' := find_valid 16 (λ width, issome (find_eorubfx_shift width D D')) 8.
+  Definition find_ubfx D D' :=
+    width ← find_ubfx_width D D';
+    lsb ← find_ubfx_lsb width D D';
+    return H_UBFX lsb width.
+  Definition find_eorubfx D D' :=
+    width ← find_eorubfx_width D D';
+    shift ← find_eorubfx_shift width D D';
+    lsb ← find_eorubfx_lsb shift width D D';
+    return H_EOR_UBFX shift lsb width.
   Definition find_hash D D' :=
-    find_ubfx_hash 1 D D'.
+    match find_ubfx D D' with
+    | Some h => Some h
+    | _ => find_eorubfx D D'
+    end.
 End Hashing.
 
-Module Order.
-  Definition t := (int * int)%type.
-  Definition leb (a b: t) := fst b <=? fst a.
-  Lemma leb_total: forall x y : t, leb x y = true \/ leb y x = true.
-  Proof. unfold leb. lia. Qed.
-End Order.
-Require Import Sorting.Mergesort.
-Module Sort := Sort Order.
-Remark iieq_dec: forall x y : int * int, {x = y} + {x <> y}.
-Proof. intros; destruct _, _. decide equality; apply eqs. Defined.
-Definition sort_uniq lst := nodup iieq_dec (Sort.sort lst).
 Section Table.
   Fixpoint assign_table h a D D' :=
     match D, D' with
@@ -66,22 +73,9 @@ Section Table.
     end.
   Definition compute_table_a h ai D D' :=
     list_of_array (assign_table h (make (hash_size h) (4*ai)) D D').
-  Function _list_of_entries entries lst n (default: int) {measure to_nat n} :=
-    if (0 <? n) then
-      match entries with
-      | e::t =>
-          if (fst e =? n-1)
-          then _list_of_entries t (snd e::lst) (n-1) default
-          else _list_of_entries entries (default::lst) (n-1) default
-      | _ => _list_of_entries entries (default::lst) (n-1) default
-      end
-    else lst.
-  Proof. all: lia. Defined.
-  Definition list_of_entries entries sz default := _list_of_entries entries nil sz default.
   Definition compute_table_m h ai D D' :=
-    let entries := (map (λ '(i, i'), (hash_func h (4*i), 4*i')) (combine D D')) in
-    let entries' := (map (λ i', (hash_func h (4*i'), 4*i')) D') in
-    let all_entries := sort_uniq (entries++entries') in
-    list_of_entries all_entries (hash_size h) (4*ai).
-
+    let entries := (map_single (λ '(i, i'), (hash_func h (4*i), 4*i')) (combine D D')) in
+    let entries' := (map_single (λ i', (hash_func h (4*i'), 4*i')) D') in
+    let m := fin_maps.list_to_map (entries++entries') in
+    map_single (fun n => iimap_lookup n m orelse ai) (iseq (hash_size h) []).
 End Table.
