extraction/extraction.v
@@ -6,11 +6,6 @@ Extract Constant array "'a" => "'a Parray.t".
 Extract Constant List.map => "(fun f l -> Parmap.parmap f (Parmap.L l))".
 Extract Constant Util.mapi => "(fun f l -> Parmap.parmapi (fun i -> f (Uint63.of_int i)) (Parmap.L l))".
 Extract Constant Util.len => "(fun x -> Uint63.of_int (List.length x))".
-Extract Constant Hash.sort_uniq => "(List.sort_uniq (fun (a1,a2) (b1,b2) ->
-  match Uint63.compare a1 a2 with
-  | 0 -> Uint63.compare b2 b1
-  | c -> c))".
-(* Extract Constant Util.maybe_map => "(fun f l -> Parmap.parmapfold f (Parmap.L l) (maybe_op List.cons) (Some []) (maybe_op List.append))". *)
 
 Set Extraction Output Directory ".".
 Extraction "Rewriter" elf_rw_polhook.
